4107056019 廖柏丞

證明：
$$
\frac{1}{2^{2k}}\Sigma_{i=0}^{2^k-1}\Sigma_{j=0}^{2^k-1}(i-j)^2 = \frac{2^{2k}-1}{6}
$$

化簡：

let $2^k=t$
$$
\frac{1}{t^2}\Sigma_{i=0}^{t-1}\Sigma_{j=0}^{t-1}(i-j)^2
$$

$$
\frac{1}{t^{2}}\Sigma_{i=0}^{t-1}\Sigma_{j=0}^{t-1}(i^2+j^2-2ij)
$$

$$
\frac{1}{t^{2}}\Bigg(\Big(t\Sigma_{i=0}^{t-1}i^2\Big)+\Big(t\Sigma_{j=0}^{t-1}j^2\Big)+\Sigma_{i=0}^{t-1}\Sigma_{j=0}^{t-1}(-2ij)\Bigg)
$$

$$
\frac{1}{t^2}\Bigg((t)(\frac{1}{6})({t-1})(t)(2t-1)\times\textcolor{blue}2-\textcolor{blue}2\times\Sigma_{i=0}^{2^t-1}\Sigma_{j=0}^{t-1}(ij)\Bigg)
$$

$$
\frac{2}{t^2}\Bigg((t)(\frac{1}{6})({t-1})(t)(2t-1)-\Sigma_{i=0}^{t-1}\Sigma_{j=0}^{t-1}(ij)\Bigg)
$$

$$
\frac{2}{t^{2}}\Bigg(\textcolor{blue}{(t)}(\frac{1}{6})\textcolor{blue}{({t-1})(t)}(2t-1)-\frac{(t-1)\textcolor{blue}{(t)(t-1)(t)}}{4}\Bigg)
$$

$$
\frac{2\cancel{(t)}\cancel{(t)}(t-1)}{\cancel{t^2}}\Big(\frac{2t-1}{6}-\frac{t-1}{4}\Big)
$$

$$
{(t-1)}\Big(\frac{2t-1}{3}-\frac{t-1}{2}\Big)
$$

$$
(t-1)\times\frac{4t-2-3t+1}{6}
$$

$$
\frac{(t-1)(t-1)}{6}
$$

$$
\frac{t^2-1}{6}
$$

代入$t=2^k$
$$
\frac{2^{2k}-1}{6}
$$

得證